Improve scalar_tac

backends/lean/Base/Primitives/Scalar.lean
@@ -709,59 +709,21 @@ def U128.ofIntCore  := @Scalar.ofIntCore .U128
 
 --  ofInt
 -- TODO: typeclass?
-def Isize.ofInt := @Scalar.ofInt .Isize
-def I8.ofInt    := @Scalar.ofInt .I8
-def I16.ofInt   := @Scalar.ofInt .I16
-def I32.ofInt   := @Scalar.ofInt .I32
-def I64.ofInt   := @Scalar.ofInt .I64
-def I128.ofInt  := @Scalar.ofInt .I128
-def Usize.ofInt := @Scalar.ofInt .Usize
-def U8.ofInt    := @Scalar.ofInt .U8
-def U16.ofInt   := @Scalar.ofInt .U16
-def U32.ofInt   := @Scalar.ofInt .U32
-def U64.ofInt   := @Scalar.ofInt .U64
-def U128.ofInt  := @Scalar.ofInt .U128
+@[reducible] def Isize.ofInt := @Scalar.ofInt .Isize
+@[reducible] def I8.ofInt    := @Scalar.ofInt .I8
+@[reducible] def I16.ofInt   := @Scalar.ofInt .I16
+@[reducible] def I32.ofInt   := @Scalar.ofInt .I32
+@[reducible] def I64.ofInt   := @Scalar.ofInt .I64
+@[reducible] def I128.ofInt  := @Scalar.ofInt .I128
+@[reducible] def Usize.ofInt := @Scalar.ofInt .Usize
+@[reducible] def U8.ofInt    := @Scalar.ofInt .U8
+@[reducible] def U16.ofInt   := @Scalar.ofInt .U16
+@[reducible] def U32.ofInt   := @Scalar.ofInt .U32
+@[reducible] def U64.ofInt   := @Scalar.ofInt .U64
+@[reducible] def U128.ofInt  := @Scalar.ofInt .U128
 
--- TODO: factor those lemmas out
 @[simp] theorem Scalar.ofInt_val_eq {ty} (h : Scalar.min ty ≤ x ∧ x ≤ Scalar.max ty) : (Scalar.ofInt x h).val = x := by
   simp [Scalar.ofInt, Scalar.ofIntCore]
-
-@[simp] theorem Isize.ofInt_val_eq (h : Scalar.min ScalarTy.Isize ≤ x ∧ x ≤ Scalar.max ScalarTy.Isize) : (Isize.ofInt x h).val = x := by
-  apply Scalar.ofInt_val_eq h
-
-@[simp] theorem I8.ofInt_val_eq (h : Scalar.min ScalarTy.I8 ≤ x ∧ x ≤ Scalar.max ScalarTy.I8) : (I8.ofInt x h).val = x := by
-  apply Scalar.ofInt_val_eq h
-
-@[simp] theorem I16.ofInt_val_eq (h : Scalar.min ScalarTy.I16 ≤ x ∧ x ≤ Scalar.max ScalarTy.I16) : (I16.ofInt x h).val = x := by
-  apply Scalar.ofInt_val_eq h
-
-@[simp] theorem I32.ofInt_val_eq (h : Scalar.min ScalarTy.I32 ≤ x ∧ x ≤ Scalar.max ScalarTy.I32) : (I32.ofInt x h).val = x := by
-  apply Scalar.ofInt_val_eq h
-
-@[simp] theorem I64.ofInt_val_eq (h : Scalar.min ScalarTy.I64 ≤ x ∧ x ≤ Scalar.max ScalarTy.I64) : (I64.ofInt x h).val = x := by
-  apply Scalar.ofInt_val_eq h
-
-@[simp] theorem I128.ofInt_val_eq (h : Scalar.min ScalarTy.I128 ≤ x ∧ x ≤ Scalar.max ScalarTy.I128) : (I128.ofInt x h).val = x := by
-  apply Scalar.ofInt_val_eq h
-
-@[simp] theorem Usize.ofInt_val_eq (h : Scalar.min ScalarTy.Usize ≤ x ∧ x ≤ Scalar.max ScalarTy.Usize) : (Usize.ofInt x h).val = x := by
-  apply Scalar.ofInt_val_eq h
-
-@[simp] theorem U8.ofInt_val_eq (h : Scalar.min ScalarTy.U8 ≤ x ∧ x ≤ Scalar.max ScalarTy.U8) : (U8.ofInt x h).val = x := by
-  apply Scalar.ofInt_val_eq h
-
-@[simp] theorem U16.ofInt_val_eq (h : Scalar.min ScalarTy.U16 ≤ x ∧ x ≤ Scalar.max ScalarTy.U16) : (U16.ofInt x h).val = x := by
-  apply Scalar.ofInt_val_eq h
-
-@[simp] theorem U32.ofInt_val_eq (h : Scalar.min ScalarTy.U32 ≤ x ∧ x ≤ Scalar.max ScalarTy.U32) : (U32.ofInt x h).val = x := by
-  apply Scalar.ofInt_val_eq h
-
-@[simp] theorem U64.ofInt_val_eq (h : Scalar.min ScalarTy.U64 ≤ x ∧ x ≤ Scalar.max ScalarTy.U64) : (U64.ofInt x h).val = x := by
-  apply Scalar.ofInt_val_eq h
-
-@[simp] theorem U128.ofInt_val_eq (h : Scalar.min ScalarTy.U128 ≤ x ∧ x ≤ Scalar.max ScalarTy.U128) : (U128.ofInt x h).val = x := by
-  apply Scalar.ofInt_val_eq h
-
 
 -- Comparisons
 instance {ty} : LT (Scalar ty) where
@@ -789,6 +751,9 @@ instance (ty : ScalarTy) : DecidableEq (Scalar ty) :=
 
 instance (ty : ScalarTy) : CoeOut (Scalar ty) Int where
   coe := λ v => v.val
+
+@[simp] theorem Scalar.neq_to_neq_val {ty} : ∀ {i j : Scalar ty}, (¬ i = j) ↔ ¬ i.val = j.val := by
+  intro i j; cases i; cases j; simp
 
 -- -- We now define a type class that subsumes the various machine integer types, so
 -- -- as to write a concise definition for scalar_cast, rather than exhaustively
